nack to Option

src/Sound/Data/Ast/Expr.dfy
@@ -36,6 +36,81 @@ module Expr {
       case LogicalNot | UnaryMinus => true
       case _ => false
     }
+
+    opaque function Eval(args: seq<M.Any>): Option<M.Any>
+    {
+      if this == IfThenElse then
+        if |args| != 3 then None
+        else 
+          var guard := args[0];
+          var thn := args[1];
+          var els := args[2];
+          if M.IsBool(guard) then 
+            if M.ToBool(guard) then Some(thn) else Some(els)
+          else None
+        else if IsUnaryOperator() then
+          if |args| != 1 then None
+          else
+            var e := args[0];
+            if M.IsBool(e) && this == LogicalNot then
+              Some(M.Not(e))
+            else if M.IsInt(e) && this == UnaryMinus then
+              Some(M.Negate(e))
+            else None
+        else if IsBinaryOperator() then
+          if |args| != 2 then None
+          else
+            var e0 := args[0];
+            var e1 := args[1];
+            match this {
+              case Eql => Some(M.InterpBool(e0 == e1))
+              case Neql => Some(M.InterpBool(e0 != e1))
+              case _ =>
+                if M.IsBool(e0) && M.IsBool(e1) then
+                  match this {
+                    case Equiv => Some(M.Equiv(e0, e1))
+                    case LogicalImp => Some(M.Implies(e0, e1))
+                    case LogicalAnd => Some(M.LogicAnd(e0, e1))
+                    case LogicalOr => Some(M.Or(e0, e1))
+                    case _ => None
+                  }
+                else if M.IsInt(e0) && M.IsInt(e1) then
+                  match this {
+                    case Less => Some(M.Less(e0, e1))
+                    case AtMost => Some(M.AtMost(e0, e1))
+                    case Plus => Some(M.Plus(e0, e1))
+                    case Minus => Some(M.Minus(e0, e1))
+                    case Times => Some(M.Times(e0, e1))
+                    case Div => Some(M.Div(e0, e1))
+                    case Mod => Some(M.Mod(e0, e1))
+                    case _ => None
+                  }
+                else None
+            }
+        else None
+    }
+  }
+
+  lemma EqlEvalLemma(v1: M.Any, v2: M.Any)
+    ensures Eql.Eval([v1, v2]) == Some(M.InterpBool(v1 == v2))
+  {
+    reveal Eql.Eval;
+  }
+
+  lemma AndEvalLemma(v1: M.Any, v2: M.Any)
+    requires M.IsBool(v1)
+    requires M.IsBool(v2)
+    ensures LogicalAnd.Eval([v1, v2]) == Some(M.LogicAnd(v1, v2))
+  {
+    reveal LogicalAnd.Eval;
+  }
+
+  lemma ImpliesEvalLemma(v1: M.Any, v2: M.Any)
+    requires M.IsBool(v1)
+    ensures LogicalImp.Eval([v1, v2]) == 
+      if M.IsBool(v2) then Some(M.Implies(v1, v2)) else None
+  {
+    reveal LogicalImp.Eval;
   }
 
   datatype Type = 
@@ -126,87 +201,32 @@ module Expr {
       Depth() <= d
     }
 
-    ghost function Eval(s: State): M.Any
+    ghost function Eval(s: State): Option<M.Any>
       requires IsDefinedOn(|s|)
-      // reads *
     {
       match this
-      case BConst(bvalue)  => M.InterpBool(bvalue)
-      case IConst(ivalue)  => M.InterpInt(ivalue)
-      case BVar(id) => s[id]
-      case CustomConst(value) => M.InterpLiteral(value.ToLiteral())
-      // ternary operators
-      case OperatorExpr(op, ss) => 
-        if op == IfThenElse then
-          if |ss| != 3 then M.Bot
-          else 
-            var guard := ss[0].Eval(s);
-            var thn := ss[1].Eval(s);
-            var els := ss[2].Eval(s);
-            if M.IsBool(guard) then 
-              if M.ToBool(guard) then thn else els
-            else M.Bot
-        else if op.IsUnaryOperator() then
-          if |ss| != 1 then M.Bot
-          else
-            var e := ss[0].Eval(s);
-            if M.IsBool(e) && op == LogicalNot then
-              M.Not(e)
-            else if M.IsInt(e) && op == UnaryMinus then
-              M.Negate(e)
-            else M.Bot
-        else if op.IsBinaryOperator() then
-          if |ss| != 2 then M.Bot
-          else
-            var e0 := ss[0].Eval(s);
-            var e1 := ss[1].Eval(s);
-            match op {
-              case Eql => M.InterpBool(e0 == e1)
-              case Neql => M.InterpBool(e0 != e1)
-              case _ =>
-                if M.IsBool(e0) && M.IsBool(e1) then
-                  match op {
-                    case Equiv => M.Equiv(e0, e1)
-                    case LogicalImp => M.Implies(e0, e1)
-                    case LogicalAnd => M.And(e0, e1)
-                    case LogicalOr => M.Or(e0, e1)
-                    case _ => M.Bot
-                  }
-                else if M.IsInt(e0) && M.IsInt(e1) then
-                  match op {
-                    case Less => M.Less(e0, e1)
-                    case AtMost => M.AtMost(e0, e1)
-                    case Plus => M.Plus(e0, e1)
-                    case Minus => M.Minus(e0, e1)
-                    case Times => M.Times(e0, e1)
-                    case Div => M.Div(e0, e1)
-                    case Mod => M.Mod(e0, e1)
-                    case _ => M.Bot
-                  }
-                else M.Bot
-            }
-        else M.Bot
+      case BConst(bvalue)  => Some(M.InterpBool(bvalue))
+      case IConst(ivalue)  => Some(M.InterpInt(ivalue))
+      case BVar(id) => Some(s[id])
+      case CustomConst(value) => Some(M.InterpLiteral(value.ToLiteral()))
+      case OperatorExpr(op, args) => 
+        var args :- SeqEval(args, s);
+        op.Eval(args)
       case FunctionCallExpr(func, args) => 
-        var args := seq(|args|, (i: nat) requires i < |args| => 
-          SeqExprDepthLemma(args, args[i]);
-          args[i].Eval(s));
-        // if func.IsUninterpreted() then
+        var args :- SeqEval(args, s);
           if func.ArgsCompatibleWith(args) then
-            M.InterpFunctionOn(func.ToFunction(), args)
-          else M.Bot
-        // else if func.GetDef().IsDefinedOn(|args|) then
-        //   func.EvalArgs(args)
-        // else M.Bot
+            Some(M.InterpFunctionOn(func.ToFunction(), args))
+          else None
       case QuantifierExpr(true, v, typ, body) =>
-        M.InterpBool(forall x: M.Any | M.HasType(x, typ.ToType()) :: 
-          body.Eval(s.Update([x])) == M.True
-        )
+        Some(M.InterpBool(forall x: M.Any | M.HasType(x, typ.ToType()) :: 
+          body.Eval(s.Update([x])) == Some(M.True)
+        ))
       case QuantifierExpr(false, v, typ, body) =>
-        M.InterpBool(exists x: M.Any | M.HasType(x, typ.ToType()) :: 
-          body.Eval(s.Update([x])) == M.True
-        )
+        Some(M.InterpBool(exists x: M.Any | M.HasType(x, typ.ToType()) :: 
+          body.Eval(s.Update([x])) == Some(M.True)
+        ))
       case LetExpr(v, rhs, body) => 
-        var x := rhs.Eval(s);
+        var x :- rhs.Eval(s);
         body.Eval(s.Update([x]))
     }
 
@@ -214,7 +234,7 @@ module Expr {
       requires IsDefinedOn(|s|)
       // reads *
     {
-      Eval(s) == M.True
+      Eval(s) == Some(M.True)
     }
 
     // lemma ForallPush(s1: State, s2: State, e1: Expr, e2: Expr, model: Model)
@@ -233,7 +253,8 @@ module Expr {
       match this
       case QuantifierExpr(true, v, tp, body) => 
       case QuantifierExpr(false, v, tp, body) => 
-      case FunctionCallExpr(func, args) => 
+      case FunctionCallExpr(func, args) => SeqEvalDepthLemma(args, s1, s2);
+      case OperatorExpr(op, args) => SeqEvalDepthLemma(args, s1, s2);
       case _ =>
     } 
 
@@ -247,6 +268,65 @@ module Expr {
       // reads *
     { 
       iset st: State | IsDefinedOn(|st|) && HoldsOn(st) 
+    }
+  }
+
+  ghost function SeqEval(ss: seq<Expr>, s: State): Option<seq<M.Any>>
+    requires forall e <- ss :: e.IsDefinedOn(|s|)
+    // ensures |SeqEval(ss, s)| == |ss|
+  {
+    if ss == [] then Some([]) else
+    var e :- ss[0].Eval(s);
+    var es :- SeqEval(ss[1..], s);
+    Some([e] + es)
+  }
+
+  lemma SeqEval1(e: Expr, s: State)
+    requires e.IsDefinedOn(|s|)
+    requires e.Eval(s).Some?
+    ensures SeqEval([e], s) == Some([e.Eval(s).value])
+  {
+    calc {
+      SeqEval([e], s);
+      == { assert [e][1..] == [];
+           assert [e][0] == e; }
+      Some([e.Eval(s).value] + []);
+      == { assert [e.Eval(s).value] + [] == [e.Eval(s).value]; }
+      Some([e.Eval(s).value]);
+    }
+  }
+
+  lemma SeqEval2(e1: Expr, e2: Expr, s: State)
+    requires e1.IsDefinedOn(|s|)
+    requires e2.IsDefinedOn(|s|)
+    requires e1.Eval(s).Some?
+    requires e2.Eval(s).Some?
+    ensures SeqEval([e1, e2], s) == Some([e1.Eval(s).value, e2.Eval(s).value])
+  {
+    assert [e1, e2][1..] == [e2];
+    assert [e1, e2][0] == e1;
+    SeqEval1(e2, s); 
+    calc {
+      SeqEval([e1, e2], s);
+      == { assert [e1, e2][1..] == [e2];
+           assert [e1, e2][0] == e1;
+           SeqEval1(e2, s); }
+      Some([e1.Eval(s).value] + SeqEval([e2], s).value);
+      == { SeqEval1(e2, s);
+           assert [e1.Eval(s).value] + [e2.Eval(s).value] == [e1.Eval(s).value, e2.Eval(s).value]; }
+      Some([e1.Eval(s).value, e2.Eval(s).value]);
+    }
+  }
+
+  lemma SeqEvalDepthLemma(ss: seq<Expr>, s1: State, s2: State)
+    requires SeqExprDepth(ss) <= |s1|
+    requires SeqExprDepth(ss) <= |s2|
+    requires forall i: Idx :: i < SeqExprDepth(ss) ==> s1[i] == s2[i]
+    ensures SeqEval(ss, s1) == SeqEval(ss, s2)
+  {
+    if ss != [] {
+      ss[0].EvalDepthLemma(s1, s2);
+      SeqEvalDepthLemma(ss[1..], s1, s2);
     }
   }
 
@@ -284,11 +364,23 @@ module Expr {
     requires e1.IsDefinedOn(|s|)
     requires e2.IsDefinedOn(|s|)
     requires e1.Eval(s) == e2.Eval(s)
+    requires e1.Eval(s).Some?
     ensures Eq(e1, e2).Depth() == max(e1.Depth(), e2.Depth())
     ensures Eq(e1, e2).IsDefinedOn(|s|)
     ensures Eq(e1, e2).HoldsOn(s)
   { 
     SeqMaxPairLemma(e1, e2);
+    calc {
+      Eq(e1, e2).Eval(s);
+      ==
+      OperatorExpr(Eql, [e1, e2]).Eval(s);
+      == { SeqEval2(e1, e2, s); }
+      Eql.Eval([e1.Eval(s).value, e2.Eval(s).value]);
+      == { EqlEvalLemma(e1.Eval(s).value, e2.Eval(s).value); }
+      Some(M.InterpBool(e1.Eval(s).value == e2.Eval(s).value));
+      == { assert e1.Eval(s) == e2.Eval(s); }
+      Some(M.InterpBool(true));
+    }
   }
 
   lemma SeqExprDepthLemma(ss: seq<Expr>, s: Expr) 
@@ -324,6 +416,8 @@ module Expr {
     ensures And(e0, e1).HoldsOn(s)
   {
     SeqMaxPairLemma(e0, e1);
+    SeqEval2(e0, e1, s);
+    AndEvalLemma(e0.Eval(s).value, e1.Eval(s).value);
   }
 
   lemma HoldsOnImpliesLemma(e0: Expr, e1: Expr, s: State)
@@ -336,17 +430,20 @@ module Expr {
     ensures e1.HoldsOn(s)
   {
     IsDefinedOnImpliesLemma(e0, e1, s);
-    M.BoolNotBot(M.True);
-    assert M.IsBool(e0.Eval(s));
-    assert M.IsBool(e1.Eval(s));
-    calc {
-      Implies(e0, e1).Eval(s);
-      ==
-      M.Implies(e0.Eval(s), e1.Eval(s));
-      ==
-      M.Implies(M.True, e1.Eval(s));
-      ==
-      M.InterpBool(true ==> M.ToBool(e1.Eval(s)));
+    assert e0.Eval(s).Some?;
+    assert SeqEval([e0, e1], s).Some?;
+    if e1.Eval(s).Some? {
+      SeqEval2(e0, e1, s);
+      calc {
+        Implies(e0, e1).Eval(s).value;
+        == { SeqEval2(e0, e1, s);
+             ImpliesEvalLemma(e0.Eval(s).value, e1.Eval(s).value); }
+        M.Implies(e0.Eval(s).value, e1.Eval(s).value);
+        ==
+        M.Implies(M.True, e1.Eval(s).value);
+        ==
+         M.InterpBool(true ==> M.ToBool(e1.Eval(s).value));
+      }
     }
   }
 
